Logic/Predicate/FirstOrder/Calculus.lean
@@ -17,19 +17,21 @@ def shifts (Δ : Finset (SyntacticSubFormula L n)) :
 @[simp] lemma shifts_ss (Δ Γ : Finset (SyntacticSubFormula L n)) :
     shifts Δ ⊆ shifts Γ ↔ Δ ⊆ Γ := Finset.map_subset_map
 
+lemma shifts_insert (p : SyntacticSubFormula L n) (Δ : Finset (SyntacticSubFormula L n)) :
+    shifts (insert p Δ) = insert (shift p) (shifts Δ) :=
+  by simp[shifts, shiftEmb_eq_shift]
+
 inductive Derivation : Finset (SyntacticFormula L) → Type _
-| AxL     : ∀ (Δ : Finset (SyntacticFormula L)) {k} (r : L.rel k) (v : Fin k → SyntacticTerm L),
+| AxL   : ∀ (Δ : Finset (SyntacticFormula L)) {k} (r : L.rel k) (v : Fin k → SyntacticTerm L),
     rel r v ∈ Δ → nrel r v ∈ Δ → Derivation Δ
-| verum   : ∀ (Δ : Finset (SyntacticFormula L)), ⊤ ∈ Δ → Derivation Δ
-| orLeft  : ∀ (Δ : Finset (SyntacticFormula L)) (p q : SyntacticFormula L),
-    Derivation (insert p Δ) → Derivation (insert (p ⋎ q) Δ)
-| orRight : ∀ (Δ : Finset (SyntacticFormula L)) (p q : SyntacticFormula L),
-    Derivation (insert q Δ) → Derivation (insert (p ⋎ q) Δ)
-| and     : ∀ (Δ : Finset (SyntacticFormula L)) (p q : SyntacticFormula L),
+| verum : ∀ (Δ : Finset (SyntacticFormula L)), ⊤ ∈ Δ → Derivation Δ
+| or  : ∀ (Δ : Finset (SyntacticFormula L)) (p q : SyntacticFormula L),
+    Derivation (insert q $ insert p Δ) → Derivation (insert (p ⋎ q) Δ)
+| and   : ∀ (Δ : Finset (SyntacticFormula L)) (p q : SyntacticFormula L),
     Derivation (insert p Δ) → Derivation (insert q Δ) → Derivation (insert (p ⋏ q) Δ)
-| all     : ∀ (Δ : Finset (SyntacticFormula L)) (p : SyntacticSubFormula L 1),
+| all   : ∀ (Δ : Finset (SyntacticFormula L)) (p : SyntacticSubFormula L 1),
     Derivation (insert (free p) (shifts Δ)) → Derivation (insert (∀' p) Δ)
-| ex      : ∀ (Δ : Finset (SyntacticFormula L)) (t : SyntacticTerm L) (p : SyntacticSubFormula L 1),
+| ex    : ∀ (Δ : Finset (SyntacticFormula L)) (t : SyntacticTerm L) (p : SyntacticSubFormula L 1),
     Derivation (insert (subst t p) Δ) → Derivation (insert (∃' p) Δ)
 
 instance : HasVdash (Finset (SyntacticFormula L)) (Type _) := ⟨Derivation⟩
@@ -46,61 +48,47 @@ section Repr
 variable [∀ k, ToString (L.func k)] [∀ k, ToString (L.rel k)]
 
 protected unsafe def repr : {Δ : Finset (SyntacticFormula L)} → Derivation Δ → String
-  | _, AxL Δ r v _ _ =>
+  | _, AxL Δ _ _ _ _ =>
       "\\AxiomC{}\n" ++
       "\\RightLabel{\\scriptsize(AxL)}\n" ++
-      "\\UnaryInfC{$\\Vdash " ++ reprStr (rel r v) ++ ", " ++ reprStr (nrel r v) ++ ", " ++
-      reprStr (Δ \ {rel r v, nrel r v}) ++ "$}\n\n"
+      "\\UnaryInfC{$\\Vdash " ++ reprStr Δ ++ "$}\n\n"
   | _, verum Δ _     =>
       "\\AxiomC{}\n" ++
-      "\\RightLabel{\\scriptsize(Verum)}\n" ++
-      "\\UnaryInfC{$\\Vdash \\top," ++ reprStr Δ ++ "$}\n\n"
-  | _, orLeft Δ p q d =>
+      "\\RightLabel{\\scriptsize($\\top$)}\n" ++
+      "\\UnaryInfC{$\\Vdash " ++ reprStr Δ ++ "$}\n\n"
+  | _, or Δ p q d =>
       d.repr ++
-      "\\RightLabel{\\scriptsize(OrLeft)}\n" ++
-      "\\UnaryInfC{$\\Vdash " ++ reprStr (p ⋎ q) ++ "," ++ reprStr Δ ++ "$}\n\n"
-  | _, orRight Δ p q d =>
-      d.repr ++
-      "\\RightLabel{\\scriptsize(OrRight)}\n" ++
-      "\\UnaryInfC{$\\Vdash " ++ reprStr (p ⋎ q) ++ "," ++ reprStr Δ ++ "$}\n\n"
+      "\\RightLabel{\\scriptsize($\\lor$)}\n" ++
+      "\\UnaryInfC{$\\Vdash " ++ reprStr (insert (p ⋎ q) Δ) ++ "$}\n\n"
   | _, and Δ p q dp dq =>
       dp.repr ++
       dq.repr ++
-      "\\RightLabel{\\scriptsize(And)}\n" ++
-      "\\BinaryInfC{$\\Vdash " ++ reprStr (p ⋏ q) ++ ", " ++ reprStr Δ ++ "$}\n\n"
+      "\\RightLabel{\\scriptsize($\\land$)}\n" ++
+      "\\BinaryInfC{$\\Vdash " ++ reprStr (insert (p ⋏ q) Δ) ++ "$}\n\n"
   | _, all Δ p d =>
       d.repr ++
-      "\\RightLabel{\\scriptsize(All)}\n" ++
-      "\\UnaryInfC{$\\Vdash" ++ reprStr (∀' p) ++ ", " ++ reprStr Δ ++ "$}\n\n"
+      "\\RightLabel{\\scriptsize($\\forall$)}\n" ++
+      "\\UnaryInfC{$\\Vdash " ++ reprStr (insert (∀' p) Δ) ++ "$}\n\n"
   | _, ex Δ _ p d =>
       d.repr ++
-      "\\RightLabel{\\scriptsize(Exists)}\n" ++
-      "\\UnaryInfC{$\\Vdash " ++ reprStr (∃' p) ++ ", " ++ reprStr Δ ++ "$}\n\n"
+      "\\RightLabel{\\scriptsize($\\exists$)}\n" ++
+      "\\UnaryInfC{$\\Vdash " ++ reprStr (insert (∃' p) Δ) ++ "$}\n\n"
 
-unsafe instance : Repr (Derivation Δ) where
+unsafe instance : Repr (⊩ Δ) where
   reprPrec d _ := d.repr
-
-def dtest := @AxL Language.equal _ _
-  { ∀' ∃' SubFormula.nrel! Language.equal 2 Language.EqRel.equal (&0 :> #1 :> Fin.nil),
-    SubFormula.rel! Language.equal 2 Language.EqRel.equal (&0 :> &1 :> Fin.nil),
-    SubFormula.nrel! Language.equal 2 Language.EqRel.equal (&0 :> &1 :> Fin.nil) }
-  2 Language.EqRel.equal (&0 :> &1 :> Fin.nil) (by simp) (by simp)
 
 end Repr
 
-protected def cast (d : ⊩ Δ) (e : Δ = Γ) : ⊩ Γ := cast (by rw[e]) d
+protected def cast (d : Derivation Δ) (e : Δ = Γ) : ⊩ Γ := cast (by simp[HasVdash.vdash, e]) d
 
 def weakening : ∀ {Δ}, ⊩ Δ → ∀ {Γ : Finset (SyntacticFormula L)}, Δ ⊆ Γ → ⊩ Γ
   | _, AxL Δ r v hrel hnrel, Γ, h => AxL Γ r v (h hrel) (h hnrel)
   | _, verum Δ htop,         Γ, h => verum Γ (h htop)
-  | _, orLeft Δ p q d,       Γ, h =>
-      have : ⊩ insert p Γ := weakening d (Finset.insert_subset_insert p (Finset.insert_subset.mp h).2)
-      have : ⊩ insert (p ⋎ q) Γ := orLeft Γ p q this
+  | _, or Δ p q d,       Γ, h =>
+      have : ⊩ insert q (insert p Γ) :=
+        weakening d (Finset.insert_subset_insert q $ Finset.insert_subset_insert p (Finset.insert_subset.mp h).2)
+      have : ⊩ insert (p ⋎ q) Γ := or Γ p q this
       Derivation.cast this (by simp; exact (Finset.insert_subset.mp h).1)
-  | _, orRight Δ p q d,      Γ, h =>
-      have : ⊩ insert q Γ := weakening d (Finset.insert_subset_insert q (Finset.insert_subset.mp h).2)
-      have : ⊩ insert (p ⋎ q) Γ := orRight Γ p q this
-      Derivation.cast this (by simp; exact (Finset.insert_subset.mp h).1)    
   | _, and Δ p q dp dq,      Γ, h =>
       have dp : ⊩ insert p Γ := weakening dp (Finset.insert_subset_insert p (Finset.insert_subset.mp h).2) 
       have dq : ⊩ insert q Γ := weakening dq (Finset.insert_subset_insert q (Finset.insert_subset.mp h).2) 
@@ -114,6 +102,41 @@ def weakening : ∀ {Δ}, ⊩ Δ → ∀ {Γ : Finset (SyntacticFormula L)}, Δ 
       have : ⊩ insert (subst t p) Γ := weakening d (Finset.insert_subset_insert _ $ by simpa using (Finset.insert_subset.mp h).2)
       have : ⊩ insert (∃' p) Γ := ex Γ t p this
       Derivation.cast this (by simp; exact (Finset.insert_subset.mp h).1)     
+
+def or' {p q : SyntacticFormula L} (h : p ⋎ q ∈ Δ) (d : ⊩ insert q (insert p Δ)) : ⊩ Δ :=
+  weakening (or Δ p q d) (by simp[Finset.insert_subset, h])
+
+def and' {p q : SyntacticFormula L} (h : p ⋏ q ∈ Δ) (dp : ⊩ insert p Δ) (dq : ⊩ insert q Δ) : ⊩ Δ :=
+  weakening (and Δ p q dp dq) (by simp[Finset.insert_subset, h])  
+
+def all' {p : SyntacticSubFormula L 1} (h : ∀' p ∈ Δ) (d : ⊩ insert (free p) (shifts Δ)) : ⊩ Δ :=
+  weakening (all Δ p d) (by simp[Finset.insert_subset, h])
+
+def ex' {p : SyntacticSubFormula L 1} (t : SyntacticTerm L) (h : ∃' p ∈ Δ)
+  (d : ⊩ insert (subst t p) Δ) : ⊩ Δ :=
+  weakening (ex Δ t p d) (by simp[Finset.insert_subset, h])
+
+def em {p : SyntacticFormula L} {Δ : Finset (SyntacticFormula L)} (hpos : p ∈ Δ) (hneg : ~p ∈ Δ) : ⊩ Δ := by
+  induction p using SubFormula.formulaRec generalizing Δ
+  case hverum    => exact verum Δ hpos
+  case hfalsum   => exact verum Δ hneg
+  case hrel r v  => exact AxL Δ r v hpos hneg 
+  case hnrel r v => exact AxL Δ r v hneg hpos 
+  case hall p ih =>
+    exact all' hpos $ ex' (p := ~ shift p) &0
+      (by simp; exact Or.inr (by simpa[-Finset.mem_map, shiftEmb_eq_shift] using Finset.mem_map_of_mem shiftEmb hneg))
+      (by simpa using ih (by simp) (by simp))
+  case hex p ih =>
+    simp at hneg
+    exact all' hneg $ ex' (p := shift p) &0
+      (by simp; exact Or.inr (by simpa[-Finset.mem_map, shiftEmb_eq_shift] using Finset.mem_map_of_mem shiftEmb hpos))
+      (by simpa using ih (by simp) (by simp))
+  case hand p q ihp ihq =>
+    simp at hneg
+    exact or' hneg $ and' (p := p) (q := q) (by simp[hpos]) (ihp (by simp) (by simp)) (ihq (by simp) (by simp))
+  case hor p q ihp ihq =>
+    simp at hneg
+    exact or' hpos $ and' (p := ~p) (q := ~q) (by simp[hneg]) (ihp (by simp) (by simp)) (ihq (by simp) (by simp))
 
 section Hom
 variable
@@ -130,14 +153,10 @@ def onDerivation (Φ : L₁ →ᵥ L₂) : ∀ {Δ : Finset (SyntacticFormula L�
       AxL _ (Φ.onRel r) (fun i => Φ.onSubTerm (v i))
         (Finset.mem_image_of_mem _ hrel) (Finset.mem_image_of_mem _ hnrel)
   | _, verum Δ h            => verum _ (by simpa using Finset.mem_image_of_mem Φ.onSubFormula₁ h)
-  | _, orLeft Δ p q d       =>
+  | _, or Δ p q d           =>
       have : ⊩ insert (Φ.onSubFormula₁ p ⋎ Φ.onSubFormula₁ q) (Finset.image Φ.onSubFormula₁ Δ) :=
-        orLeft _ _ _ (Derivation.cast (onDerivation Φ d) (by simp))
+        or _ _ _ (Derivation.cast (onDerivation Φ d) (by simp))
       Derivation.cast this (by simp)
-  | _, orRight Δ p q d      =>
-      have : ⊩ insert (Φ.onSubFormula₁ p ⋎ Φ.onSubFormula₁ q) (Finset.image Φ.onSubFormula₁ Δ) :=
-        orRight _ _ _ (Derivation.cast (onDerivation Φ d) (by simp))
-      Derivation.cast this (by simp) 
   | _, and Δ p q dp dq      =>
       have : ⊩ insert (Φ.onSubFormula₁ p ⋏ Φ.onSubFormula₁ q) (Finset.image Φ.onSubFormula₁ Δ) :=
         and _ _ _ (Derivation.cast (onDerivation Φ dp) (by simp)) (Derivation.cast (onDerivation Φ dq) (by simp))
@@ -165,13 +184,74 @@ def decomp : Finset (SyntacticTerm L) → SyntacticFormula L → Finset (Syntact
 | _, ∀' p,     Γ => some { insert (SubFormula.free p) (shifts Γ) }
 | s, ∃' p,     Γ => some { s.image (subst · p) ∪ Γ }
 
-#check SubFormula.rel! Language.equal 2 Language.EqRel.equal (#0 :> #0 :> Fin.nil)
+def exOfInstances (v : List (SyntacticTerm L)) (p : SyntacticSubFormula L 1)
+  (h : ⊩ (v.map (subst · p)).toFinset ∪ Γ) : ⊩ insert (∃' p) Γ := by
+  induction' v with t v ih generalizing Γ <;> simp at h
+  · exact weakening h (Finset.subset_insert _ Γ)
+  · exact Derivation.cast (ih (Γ := insert (∃' p) Γ)
+      (Derivation.cast (ex _ t p h) (by ext r; simp))) (by simp)
 
-#eval SubTerm.toNat (SubTerm.func! (μ := ℕ) (n := 0) Language.ring 2 Language.RingFunc.add (&0 :> &1 :> Fin.nil))
+
+def deriveList? (tmax : ℕ) : ℕ → (Γ : List (SyntacticFormula L)) → Option (⊩ Γ.toFinset)
+  | 0,     _      => none
+  | _ + 1, []     => none
+  | s + 1, p :: Γ => if h : ~p ∈ Γ then some (em (p := p) (by simp) (by simp[h]))
+      else match p with
+      | ⊤        => some $ verum _ (by simp)
+      | ⊥        => (deriveList? tmax s Γ).map (fun d => weakening d (by simpa using Finset.subset_insert ⊥ Γ.toFinset))
+      | rel r v  => (deriveList? tmax s $ Γ ++ [rel r v]).map (fun d => d.cast $ by ext; simp; tauto)
+      | nrel r v => (deriveList? tmax s $ Γ ++ [nrel r v]).map (fun d => d.cast $ by ext; simp; tauto)
+      | p ⋎ q    => (deriveList? tmax s (Γ ++ [p, q])).map
+          fun d => (or Γ.toFinset p q (d.cast $ by ext; simp; tauto)).cast (by ext; simp)
+      | p ⋏ q    => (deriveList? tmax s (Γ ++ [p])).bind fun dp => (deriveList? tmax s (Γ ++ [q])).map
+          fun dq => (and Γ.toFinset p q (dp.cast $ by ext; simp[or_comm]) (dq.cast $ by ext; simp[or_comm])).cast 
+            (by ext; simp[or_comm])
+      | ∀' p     => (deriveList? tmax s (Γ.map shift ++ [free p])).map
+          fun d => (all (Γ.toFinset) p (d.cast $ by ext; simp[shifts, shiftEmb, or_comm])).cast (by simp)
+      | ∃' p     => (deriveList? tmax s (Γ ++ [∃' p] ++ (SubTerm.enumLtList tmax).map (subst · p))).map
+          fun d => (exOfInstances (Γ := insert (∃' p) Γ.toFinset) (SubTerm.enumLtList tmax)
+            p (d.cast $ by ext; simp[or_comm])).cast (by ext; simp)
+
+def derive? (tmax s : ℕ) (p : SyntacticFormula L) : Option (⊩ ({p} : Finset (SyntacticFormula L))) :=
+  deriveList? tmax s [p]
 
 
-#eval @instanceEnum Language.ring _ _ _
-  (SubFormula.rel! Language.ring 2 Language.RingRel.le (#0 :> #0 :> Fin.nil)) 2
+variable (p q : SyntacticFormula Language.equal)
+
+#eval derive? 8 32 (L := Language.equal) 
+  (SubFormula.rel! Language.equal 2 Language.EqRel.equal ![&0, &1] ⟶
+   (∃' ∃' SubFormula.rel! Language.equal 2 Language.EqRel.equal ![#0, #1]))
+
+#eval derive? 32 32 (L := Language.equal) 
+  (SubFormula.rel! Language.equal 2 Language.EqRel.equal ![&0, &1] ⟶
+   (∃' ∃' SubFormula.rel! Language.equal 2 Language.EqRel.equal ![#0, #1]))
+
+#eval derive? 32 32 (L := Language.equal) 
+  ((∀' ∀' SubFormula.rel! Language.equal 2 Language.EqRel.equal ![#0, #1]) ⋎
+   (∃' ∃' ~ SubFormula.rel! Language.equal 2 Language.EqRel.equal ![#0, #1]))
+
+#eval derive? 32 32 (L := Language.relational (fun _ => ℕ)) 
+  ((( SubFormula.rel! (Language.relational (fun _ => ℕ)) 0 0 ![] ⟶ 
+      SubFormula.rel! (Language.relational (fun _ => ℕ)) 0 1 ![]) ⟶
+    SubFormula.rel! (Language.relational (fun _ => ℕ)) 0 0 ![]) ⟶
+  SubFormula.rel! (Language.relational (fun _ => ℕ)) 0 0 ![])
+
+#eval derive? 32 32 (L := Language.relational (fun _ => ℕ)) 
+  ((( SubFormula.rel! (Language.relational (fun _ => ℕ)) 0 0 ![] ⋎
+      SubFormula.rel! (Language.relational (fun _ => ℕ)) 0 1 ![]) ⟶
+    ( SubFormula.rel! (Language.relational (fun _ => ℕ)) 0 1 ![] ⋎
+      SubFormula.rel! (Language.relational (fun _ => ℕ)) 0 0 ![])))
+
+#eval derive? 4 32 (L := Language.relational (fun _ => ℕ)) 
+  (∀' ( SubFormula.rel! (Language.relational (fun _ => ℕ)) 1 0 ![#0] ⋎
+        SubFormula.rel! (Language.relational (fun _ => ℕ)) 1 1 ![#0]) ⟶
+   ∀' ( SubFormula.rel! (Language.relational (fun _ => ℕ)) 1 1 ![#0] ⋎
+        SubFormula.rel! (Language.relational (fun _ => ℕ)) 1 0 ![#0]))
+
+
+#eval derive? 4 32 (L := Language.relational (fun _ => ℕ)) 
+  ( ∀'(SubFormula.rel! (Language.relational (fun _ => ℕ)) 1 0 ![#0] ⟶
+    ∃' SubFormula.rel! (Language.relational (fun _ => ℕ)) 1 0 ![#0]))
 
 end Derivation
 
